traced/utlc_traced.v
@@ -9,41 +9,32 @@ Require Import Lia.
 
 Module renSubst.
 
-
 Notation upT vs := (0 :: vs).
 
-(* Inductive fin : list nat -> Type := *)
-(*   | finO : fin [0] *)
-(*   | finS : forall l, fin l -> fin (List.map S l) *)
-(*   | finU : forall l, fin l -> fin (upT l). *)
+(** Definition of finite type based on lists.
+    It's very similar to the normal fin type of wellscoped syntax. 
+    Maybe even too much. I'm havin doubts that this is an appropriate
+    formalization of traced syntax. *)
+Inductive wrapNat (n:nat) : Type := wrapC : wrapNat n.
 
-(* Arguments finS {l}. *)
-(* Arguments finU {l}. *)
-
-(* should be able to represent any number in an ordered list *)
-(* wait that does not really work *)
-(* Check finO. *)
-(* Check finS finO : fin [1]. *)
-(* Check finU (finS finO) : fin [0;2]. *)
-
-
-Inductive fin : list nat -> Type :=
-  | finH : forall n l, fin (n::l) (* the position in the list *)
-  | finT : forall n l, fin l -> fin (n::l). (* how big the jump is to the next number *)
-
-Arguments finH _ {l}.
-Arguments finT _ {l}.
-
-Fixpoint denote {l: list nat} (x: fin l) : nat :=
-  match x with
-  | finH n => n
-  | finT n x' => n + S (denote x')
+Fixpoint fin (l: list nat) : Type :=
+  match l with
+  | [] => False
+  | n :: l => (wrapNat n) + (fin l)
   end.
 
-(* flatten [0;1;2] -> [0;0;0]
- * flatten [0;2;3] -> [0;1;0]
- * flatten [1;2;3] -> [1;0;0]
- * flatten [0;3;5] -> [0;2;1] *)
+(* compute the natural number that a value of type fin l denotes. *)
+Fixpoint denote {l: list nat} (x: fin l) {struct l} : nat.
+Proof.
+  destruct l as [|n l'].
+  - destruct x.
+  - refine (match x with
+            | inl (wrapC _) => n
+            | inr x' => S (denote l' x')
+            end).
+Defined.
+
+(* compute a "flattened" list, i.e. with the simplification which only tracks differences between the elements. *)
 Fixpoint flatten (l: list nat) (acc: nat) : list nat :=
   match l with
   | [] => []
@@ -51,89 +42,88 @@ Fixpoint flatten (l: list nat) (acc: nat) : list nat :=
     let x' := x - acc in
     x' :: flatten l (S x)
   end.
+
+(* some values of the finite type *)
 Definition fl (l: list nat) : list nat := flatten l 0.
-
-Compute (fl [0]).
-Compute (fl [0;1;2]).
-Compute (fl [0;2;3]).
-Compute (fl [1;2;3]).
-Compute (fl [0;3;5]).
-
-Definition f0 : fin (fl [0]) := finH 0.
-Definition f1 : fin (fl [0;2;3]) := finH 0. (* denotes 0 *)
-Definition f2 : fin (fl [0;2;3]) := finT 0 (finH 1). (* denotes 2 *)
-Definition f3 : fin (fl [0;2;3]) := finT 0 (finT 1 (finH 0)). (* denotes 3 *)
+Definition f0 : fin [0] := inl (wrapC 0).
+Definition f1 : fin (fl [0;2;3]) := inl (wrapC 0). (* denotes 0 *)
+Definition f2 : fin (fl [0;2;3]) := inr (inl (wrapC 1)). (* denotes 2 *)
+Definition f3 : fin (fl [0;2;3]) := inr (inr (inl (wrapC 0))). (* denotes 3 *)
 
 Compute (denote f0).
 Compute (denote f1).
 Compute (denote f2).
 Compute (denote f3).
 
-
+(* language definition *)
 Inductive tm (vs : list nat) : Type :=
   | var_tm : fin vs -> tm vs
   | app : tm vs -> tm vs -> tm vs
   | lam : tm (upT vs) -> tm vs.
-Arguments var_tm {vs}.
-Arguments app {vs}.
-Arguments lam {vs}.
 
+(* congruence lemmas are unchanged except list scope variable *)
 Lemma congr_app {vs : list nat} {s0 : tm vs} {s1 : tm vs} {t0 : tm vs}
   {t1 : tm vs} (H0 : s0 = t0) (H1 : s1 = t1) :
-  app s0 s1 = app t0 t1.
+  app _ s0 s1 = app _ t0 t1.
 Proof.
-exact (eq_trans (eq_trans eq_refl (ap (fun x => app x s1) H0))
-         (ap (fun x => app t0 x) H1)).
+exact (eq_trans (eq_trans eq_refl (ap (fun x => app _ x s1) H0))
+         (ap (fun x => app _ t0 x) H1)).
 Qed.
 
 Lemma congr_lam {vs : list nat} {s0 : tm (upT vs)} {t0 : tm (upT vs)}
-  (H0 : s0 = t0) : lam s0 = lam t0.
+  (H0 : s0 = t0) : lam _ s0 = lam _ t0.
 Proof.
-exact (eq_trans eq_refl (ap (fun x => lam x) H0)).
+exact (eq_trans eq_refl (ap (fun x => lam _ x) H0)).
 Qed.
 
 
-(* Inductive finList3 : list nat -> Type := *)
-(*     list0 : forall l, finList3 (0::l) *)
-(*   | listC : forall (v w:nat) (vs: list nat), finList3 (v::vs) -> finList3 (S v :: List.map S vs) *)
-(*   | listT : forall v vs, finList3 vs -> finList3 (v::vs). *)
-
 Open Scope type.
 
+(* scons is the biggest problem when we map S over the list.
+ * because we have to take the m, which is mapped, and pass it to f, which does not want the map.
+ * With my simplification it works fine. *)
 Definition scons {X : Type} {vs : list nat} (x : X) (f : fin vs -> X) (m : fin (upT vs)) : X.
 Proof.
-  revert m.
-  enough (H: forall vs' (Heq: vs' = upT vs), fin vs' -> X).
-  - intros m. exact (H (upT vs) eq_refl m).
-  - intros vs' Heq m.
-    destruct m.
-    + exact x.
-    + injection Heq.
-      intros -> _.
-      exact (f m).
+  destruct m as [n|m'].
+  - exact x.
+  - exact (f m').
 Defined.
 
 Compute (@scons nat (fl [1;2]) 1 (fun _ => 6) f1).
 Compute (@scons nat (fl [1;2]) 1 (fun _ => 6) f2).
 Compute (@scons nat (fl [1;2]) 1 (fun _ => 6) f3).
 
-Definition var_zero {vs: list nat} : fin (upT vs) := finH 0.
+(* we can define "lossy" primitives.  *)
+Definition var_zero {vs: list nat} : fin (upT vs) := inl (wrapC 0).
+Definition shift {vs: list nat} : fin vs -> fin (upT vs) := inr.
 
-Definition shift {vs: list nat} : fin vs -> fin (upT vs) := finT 0.
-
-Definition up_ren_traced {vs0 vs1 : list nat} (xi: fin vs0 -> fin vs1) : fin (upT vs0) -> fin (upT vs1) :=
+(* with traced syntax we can know that var_zero is in fin [0] and shift does not contain a 0
+ * but these non-lossy versions are not easy to use. *)
+Definition var_zero' : fin [0] := inl (wrapC 0).
+Definition shift' {vs: list nat} : fin vs -> fin (List.map S vs).
+Proof.
+  intros m. induction vs as [|v vs].
+  - destruct m.
+  - destruct m as [n|m'].
+    + left. constructor.
+    + right. exact (IHvs m').
+Defined.  
+ 
+Definition up_ren {m n} (xi : fin m -> fin n) : fin (upT m) -> fin (upT n) :=
   scons var_zero (funcomp shift xi).
+
+Definition upRen_tm_tm {vs0 vs1 : list nat} (xi: fin vs0 -> fin vs1) : fin (upT vs0) -> fin (upT vs1) := up_ren xi.
 
 Fixpoint ren_tm {vs0 vs1: list nat} (xi_tm : fin vs0 -> fin vs1) (s: tm vs0) {struct s} : tm vs1.
 Proof.
   refine (match s with
-          | var_tm x => _
-          | app s0 s1 => _
-          | lam s0 => _
+          | var_tm _ x => _
+          | app _ s0 s1 => _
+          | lam _ s0 => _
           end).
-  - exact (var_tm (xi_tm x)).
-  - exact (app (ren_tm _ _ xi_tm s0) (ren_tm _ _ xi_tm s1)).
-  - exact (lam (ren_tm _ _ (up_ren_traced xi_tm) s0)).
+  - exact (var_tm _ (xi_tm x)).
+  - exact (app _ (ren_tm _ _ xi_tm s0) (ren_tm _ _ xi_tm s1)).
+  - exact (lam _ (ren_tm _ _ (upRen_tm_tm xi_tm) s0)).
 Defined.
 
 Print Assumptions ren_tm.
@@ -148,13 +138,13 @@ Fixpoint subst_tm {vs0 : list nat} {vs1 : list nat} (sigma_tm : fin vs0 -> tm vs
   : tm vs1.
 Proof.
   refine (match s with
-          | var_tm x => _
-          | app s0 s1 => _
-          | lam s0 => _
+          | var_tm _ x => _
+          | app _ s0 s1 => _
+          | lam _ s0 => _
           end).
   - exact (sigma_tm x).
-  - exact (app (subst_tm _ _ sigma_tm s0) (subst_tm _ _ sigma_tm s1)).
-  - exact (lam (subst_tm _ _ (up_tm_tm sigma_tm) s0)).
+  - exact (app _ (subst_tm _ _ sigma_tm s0) (subst_tm _ _ sigma_tm s1)).
+  - exact (lam _ (subst_tm _ _ (up_tm_tm sigma_tm) s0)).
 Defined.
 
 Print Assumptions subst_tm.
@@ -163,16 +153,16 @@ Print Assumptions subst_tm.
 (* lambda . lambda . 1 2 (lambda . 3 0 1) *)
 Definition testtm : tm [1].
 Proof.
-  refine (lam (lam (app (app (* x w *) _ _)
-                        (lam (app (app (* w z *) _ _) (* y *) _))))).
+  refine (lam _ (lam _ (app _ (app _ (* x w *) _ _)
+                        (lam _ (app _ (app _ (* w z *) _ _) (* y *) _))))).
   - (* x *)
     cbv.
     (* apparently here Coq's unification is too weak *)
-    refine (@var_tm [0;0;1] var_zero).
+    refine (@var_tm (fl [0;1;3]) var_zero).
   - (* outer w *)
-    refine (@var_tm [0;0;1] (shift var_zero)).
+    refine (@var_tm (fl [0;1;3]) (shift var_zero)).
   - (* inner w *)
-    refine (@var_tm [0;0;0;1] (shift (shift var_zero))).
+    refine (@var_tm (fl [0;1;2;4]) (shift (shift var_zero))).
   - (* z *)
     exact (@var_tm (fl [0;1;2;4]) var_zero).
   - (* y *)
@@ -181,8 +171,14 @@ Defined.
 
 Print Assumptions testtm.
 Print testtm.
+
+(* and here we see that the formalization is bad. we should have enough information that a shift increases the only free variable.
+   so the type should be tm [2], but we are essentially throwing that info away. *)
+Fail Check (ren_tm shift testtm : tm [2]).
+Check (ren_tm shift testtm : tm [0;1]).
+(* we can compute with these definitions *)
 Compute (ren_tm shift testtm).
-Compute (subst_tm var_tm testtm).
+Compute (subst_tm (var_tm _) testtm).
 
 Definition ap {X Y} (f : X -> Y) {x y : X} (p : x = y) : f x = f y :=
   match p with eq_refl => eq_refl end.
@@ -191,155 +187,41 @@ Definition cast {X} {x y: X} {p: X -> Type}
   : x = y -> p x -> p y
   := fun e a => match e with eq_refl => a end.
 
-(* Lemma In_0 : forall vs (H: InN 0 (upT vs)), H = InNCons. *)
-
-Require Import Eqdep_dec.
-Module DecList <: DecidableType.
-  Definition U := list nat.
-  Definition eq_dec (x y: list nat) :=
-    list_eq_dec Nat.eq_dec x y.
-End DecList.
-
-Module UIPList := DecidableEqDep DecList.
-Lemma UIP_list (l : list nat) (e: l = l) : e = eq_refl.
-Proof.
-  apply (UIPList.UIP_refl l e).
-Qed.
-
-(* Lemma up_helper (vs: list nat) (F: forall vs, fin vs -> Prop) *)
-(*       (H0: F (upT vs) (finH 0)) *)
-(*       (H1: forall x, F (upT vs) (finT 0 x)) *)
-(*       : forall (x: fin (upT vs)), F _ x. *)
-(* Proof. *)
-(*   enough (He: forall vs' (Heq: vs' = upT vs) (x: fin vs'), F vs' x). *)
-(*   - intros x. apply (He (upT vs) eq_refl x). *)
-(*   - intros vs' Heq x. *)
-(*     destruct x. *)
-(*     + injection Heq. *)
-(*       intros -> ->. *)
-(*       apply H0. *)
-(*     + injection Heq. *)
-(*       intros -> ->. *)
-(*       apply H1. *)
-(* Qed. *)
-         
 Lemma upId_tm_tm {vs : list nat} (sigma : fin vs -> tm vs)
-  (Eq : forall x, sigma x = var_tm x) :
+  (Eq : forall x, sigma x = var_tm _ x) :
   forall x, up_tm_tm sigma x = @var_tm (upT vs) x.
 Proof.
-  unfold up_tm_tm.
-  enough (He: forall vs' (Heq: vs' = upT vs) (x : fin vs'), scons (var_tm var_zero) (funcomp (ren_tm shift) sigma) (cast Heq x) = var_tm (cast Heq x)).
-  - apply (He (upT vs) eq_refl).
-  - intros vs' Heq x.
-    destruct x.
-    + injection Heq.
-      intros -> ->.
-      rewrite (UIP_list _ Heq).
-      reflexivity.
-    + injection Heq.
-      intros -> ->.
-      rewrite (UIP_list _ Heq).
-      cbn.
-      exact (ap (ren_tm shift) (Eq x)).
+  refine (fun x =>
+          match x with
+          | inr x' => ap (ren_tm shift) (Eq x')
+          | inl (wrapC _) => eq_refl
+          end).
 Qed.
 
 Fixpoint idSubst_tm {vs : list nat} (sigma_tm : fin vs -> tm vs)
-(Eq_tm : forall x, sigma_tm x = var_tm x) (s : tm vs) {struct s} :
+(Eq_tm : forall x, sigma_tm x = var_tm _ x) (s : tm vs) {struct s} :
 subst_tm sigma_tm s = s :=
   match s as s0 return subst_tm sigma_tm s0 = s0
   with
-  | var_tm s0 => Eq_tm s0
-  | app s0 s1 => congr_app (idSubst_tm sigma_tm Eq_tm s0) (idSubst_tm sigma_tm Eq_tm s1)
-  | lam s0 => congr_lam (idSubst_tm (up_tm_tm sigma_tm) (upId_tm_tm sigma_tm Eq_tm) s0)
-  end.
-
-Fail Check 1.
-(* Lemma upRen_tm_tm {m : nat} {n : nat} (xi : fin m -> fin n) : *)
-(*   fin (S m) -> fin (S n). *)
-(* Proof. *)
-(* exact (up_ren xi). *)
-(* Defined. *)
-
-(* Fixpoint ren_tm {m_tm : nat} {n_tm : nat} (xi_tm : fin m_tm -> fin n_tm) *)
-(* (s : tm m_tm) {struct s} : tm n_tm := *)
-(*   match s with *)
-(*   | var_tm _ s0 => var_tm n_tm (xi_tm s0) *)
-(*   | app _ s0 s1 => app n_tm (ren_tm xi_tm s0) (ren_tm xi_tm s1) *)
-(*   | lam _ s0 => lam n_tm (ren_tm (upRen_tm_tm xi_tm) s0) *)
-(*   end. *)
-
-Lemma up_tm_tm {m : nat} {n_tm : nat} (sigma : fin m -> tm n_tm) :
-  fin (S m) -> tm (S n_tm).
-Proof.
-exact (scons (var_tm (S n_tm) var_zero) (funcomp (ren_tm shift) sigma)).
-Defined.
-
-Lemma up_list_tm_tm (p : nat) {m : nat} {n_tm : nat}
-  (sigma : fin m -> tm n_tm) : fin (plus p m) -> tm (plus p n_tm).
-Proof.
-exact (scons_p p (funcomp (var_tm (plus p n_tm)) (zero_p p))
-         (funcomp (ren_tm (shift_p p)) sigma)).
-Defined.
-
-Fixpoint subst_tm {m_tm : nat} {n_tm : nat} (sigma_tm : fin m_tm -> tm n_tm)
-(s : tm m_tm) {struct s} : tm n_tm :=
-  match s with
-  | var_tm _ s0 => sigma_tm s0
-  | app _ s0 s1 => app n_tm (subst_tm sigma_tm s0) (subst_tm sigma_tm s1)
-  | lam _ s0 => lam n_tm (subst_tm (up_tm_tm sigma_tm) s0)
-  end.
-
-Lemma upId_tm_tm {m_tm : nat} (sigma : fin m_tm -> tm m_tm)
-  (Eq : forall x, sigma x = var_tm m_tm x) :
-  forall x, up_tm_tm sigma x = var_tm (S m_tm) x.
-Proof.
-exact (fun n =>
-       match n with
-       | Some fin_n => ap (ren_tm shift) (Eq fin_n)
-       | None => eq_refl
-       end).
-Qed.
-
-Lemma upId_list_tm_tm {p : nat} {m_tm : nat} (sigma : fin m_tm -> tm m_tm)
-  (Eq : forall x, sigma x = var_tm m_tm x) :
-  forall x, up_list_tm_tm p sigma x = var_tm (plus p m_tm) x.
-Proof.
-exact (fun n =>
-       scons_p_eta (var_tm (plus p m_tm))
-         (fun n => ap (ren_tm (shift_p p)) (Eq n)) (fun n => eq_refl)).
-Qed.
-
-Fixpoint idSubst_tm {m_tm : nat} (sigma_tm : fin m_tm -> tm m_tm)
-(Eq_tm : forall x, sigma_tm x = var_tm m_tm x) (s : tm m_tm) {struct s} :
-subst_tm sigma_tm s = s :=
-  match s with
   | var_tm _ s0 => Eq_tm s0
-  | app _ s0 s1 =>
-      congr_app (idSubst_tm sigma_tm Eq_tm s0) (idSubst_tm sigma_tm Eq_tm s1)
-  | lam _ s0 =>
-      congr_lam (idSubst_tm (up_tm_tm sigma_tm) (upId_tm_tm _ Eq_tm) s0)
+  | app _ s0 s1 => congr_app (idSubst_tm sigma_tm Eq_tm s0) (idSubst_tm sigma_tm Eq_tm s1)
+  | lam _ s0 => congr_lam (idSubst_tm (up_tm_tm sigma_tm) (upId_tm_tm sigma_tm Eq_tm) s0)
   end.
 
-Lemma upExtRen_tm_tm {m : nat} {n : nat} (xi : fin m -> fin n)
+
+Lemma upExtRen_tm_tm {m : list nat} {n : list nat} (xi : fin m -> fin n)
   (zeta : fin m -> fin n) (Eq : forall x, xi x = zeta x) :
   forall x, upRen_tm_tm xi x = upRen_tm_tm zeta x.
 Proof.
 exact (fun n =>
        match n with
-       | Some fin_n => ap shift (Eq fin_n)
-       | None => eq_refl
+       | inr x' => ap shift (Eq x')
+       | inl n => match n with wrapC _ => eq_refl end
        end).
 Qed.
 
-Lemma upExtRen_list_tm_tm {p : nat} {m : nat} {n : nat} (xi : fin m -> fin n)
-  (zeta : fin m -> fin n) (Eq : forall x, xi x = zeta x) :
-  forall x, upRen_list_tm_tm p xi x = upRen_list_tm_tm p zeta x.
-Proof.
-exact (fun n =>
-       scons_p_congr (fun n => eq_refl) (fun n => ap (shift_p p) (Eq n))).
-Qed.
 
-Fixpoint extRen_tm {m_tm : nat} {n_tm : nat} (xi_tm : fin m_tm -> fin n_tm)
+Fixpoint extRen_tm {m_tm : list nat} {n_tm : list nat} (xi_tm : fin m_tm -> fin n_tm)
 (zeta_tm : fin m_tm -> fin n_tm) (Eq_tm : forall x, xi_tm x = zeta_tm x)
 (s : tm m_tm) {struct s} : ren_tm xi_tm s = ren_tm zeta_tm s :=
   match s with
@@ -353,28 +235,19 @@ Fixpoint extRen_tm {m_tm : nat} {n_tm : nat} (xi_tm : fin m_tm -> fin n_tm)
            (upExtRen_tm_tm _ _ Eq_tm) s0)
   end.
 
-Lemma upExt_tm_tm {m : nat} {n_tm : nat} (sigma : fin m -> tm n_tm)
+  
+Lemma upExt_tm_tm {m : list nat} {n_tm : list nat} (sigma : fin m -> tm n_tm)
   (tau : fin m -> tm n_tm) (Eq : forall x, sigma x = tau x) :
   forall x, up_tm_tm sigma x = up_tm_tm tau x.
 Proof.
 exact (fun n =>
        match n with
-       | Some fin_n => ap (ren_tm shift) (Eq fin_n)
-       | None => eq_refl
+       | inr fin_n => ap (ren_tm shift) (Eq fin_n)
+       | inl n => match n with wrapC _ => eq_refl end
        end).
 Qed.
 
-Lemma upExt_list_tm_tm {p : nat} {m : nat} {n_tm : nat}
-  (sigma : fin m -> tm n_tm) (tau : fin m -> tm n_tm)
-  (Eq : forall x, sigma x = tau x) :
-  forall x, up_list_tm_tm p sigma x = up_list_tm_tm p tau x.
-Proof.
-exact (fun n =>
-       scons_p_congr (fun n => eq_refl)
-         (fun n => ap (ren_tm (shift_p p)) (Eq n))).
-Qed.
-
-Fixpoint ext_tm {m_tm : nat} {n_tm : nat} (sigma_tm : fin m_tm -> tm n_tm)
+Fixpoint ext_tm {m_tm : list nat} {n_tm : list nat} (sigma_tm : fin m_tm -> tm n_tm)
 (tau_tm : fin m_tm -> tm n_tm) (Eq_tm : forall x, sigma_tm x = tau_tm x)
 (s : tm m_tm) {struct s} : subst_tm sigma_tm s = subst_tm tau_tm s :=
   match s with
@@ -388,7 +261,17 @@ Fixpoint ext_tm {m_tm : nat} {n_tm : nat} (sigma_tm : fin m_tm -> tm n_tm)
            s0)
   end.
 
-Lemma up_ren_ren_tm_tm {k : nat} {l : nat} {m : nat} (xi : fin k -> fin l)
+Lemma up_ren_ren (k l m : list nat) (xi: fin k -> fin l) (zeta : fin l -> fin m) (rho: fin k -> fin m) (E: forall x, (funcomp zeta xi) x = rho x) :
+  forall x, up_ren zeta (up_ren xi x) = up_ren rho x.
+Proof.
+  intros [n|x'].
+  - reflexivity.
+  - cbn. unfold funcomp. now rewrite <- E.
+Qed.
+
+Arguments up_ren_ren {k l m} xi zeta rho E.
+
+Lemma up_ren_ren_tm_tm {k : list nat} {l : list nat} {m : list nat} (xi : fin k -> fin l)
   (zeta : fin l -> fin m) (rho : fin k -> fin m)
   (Eq : forall x, funcomp zeta xi x = rho x) :
   forall x, funcomp (upRen_tm_tm zeta) (upRen_tm_tm xi) x = upRen_tm_tm rho x.
@@ -396,17 +279,7 @@ Proof.
 exact (up_ren_ren xi zeta rho Eq).
 Qed.
 
-Lemma up_ren_ren_list_tm_tm {p : nat} {k : nat} {l : nat} {m : nat}
-  (xi : fin k -> fin l) (zeta : fin l -> fin m) (rho : fin k -> fin m)
-  (Eq : forall x, funcomp zeta xi x = rho x) :
-  forall x,
-  funcomp (upRen_list_tm_tm p zeta) (upRen_list_tm_tm p xi) x =
-  upRen_list_tm_tm p rho x.
-Proof.
-exact (up_ren_ren_p Eq).
-Qed.
-
-Fixpoint compRenRen_tm {k_tm : nat} {l_tm : nat} {m_tm : nat}
+Fixpoint compRenRen_tm {k_tm : list nat} {l_tm : list nat} {m_tm : list nat}
 (xi_tm : fin m_tm -> fin k_tm) (zeta_tm : fin k_tm -> fin l_tm)
 (rho_tm : fin m_tm -> fin l_tm)
 (Eq_tm : forall x, funcomp zeta_tm xi_tm x = rho_tm x) (s : tm m_tm) {struct
@@ -422,34 +295,19 @@ Fixpoint compRenRen_tm {k_tm : nat} {l_tm : nat} {m_tm : nat}
            (upRen_tm_tm rho_tm) (up_ren_ren _ _ _ Eq_tm) s0)
   end.
 
-Lemma up_ren_subst_tm_tm {k : nat} {l : nat} {m_tm : nat}
+Lemma up_ren_subst_tm_tm {k : list nat} {l : list nat} {m_tm : list nat}
   (xi : fin k -> fin l) (tau : fin l -> tm m_tm) (theta : fin k -> tm m_tm)
   (Eq : forall x, funcomp tau xi x = theta x) :
   forall x, funcomp (up_tm_tm tau) (upRen_tm_tm xi) x = up_tm_tm theta x.
 Proof.
 exact (fun n =>
        match n with
-       | Some fin_n => ap (ren_tm shift) (Eq fin_n)
-       | None => eq_refl
+       | inr fin_n => ap (ren_tm shift) (Eq fin_n)
+       | inl n => match n with wrapC _ => eq_refl end
        end).
 Qed.
 
-Lemma up_ren_subst_list_tm_tm {p : nat} {k : nat} {l : nat} {m_tm : nat}
-  (xi : fin k -> fin l) (tau : fin l -> tm m_tm) (theta : fin k -> tm m_tm)
-  (Eq : forall x, funcomp tau xi x = theta x) :
-  forall x,
-  funcomp (up_list_tm_tm p tau) (upRen_list_tm_tm p xi) x =
-  up_list_tm_tm p theta x.
-Proof.
-exact (fun n =>
-       eq_trans (scons_p_comp' _ _ _ n)
-         (scons_p_congr (fun z => scons_p_head' _ _ z)
-            (fun z =>
-             eq_trans (scons_p_tail' _ _ (xi z))
-               (ap (ren_tm (shift_p p)) (Eq z))))).
-Qed.
-
-Fixpoint compRenSubst_tm {k_tm : nat} {l_tm : nat} {m_tm : nat}
+Fixpoint compRenSubst_tm {k_tm : list nat} {l_tm : list nat} {m_tm : list nat}
 (xi_tm : fin m_tm -> fin k_tm) (tau_tm : fin k_tm -> tm l_tm)
 (theta_tm : fin m_tm -> tm l_tm)
 (Eq_tm : forall x, funcomp tau_tm xi_tm x = theta_tm x) (s : tm m_tm) {struct
@@ -465,7 +323,7 @@ Fixpoint compRenSubst_tm {k_tm : nat} {l_tm : nat} {m_tm : nat}
            (up_tm_tm theta_tm) (up_ren_subst_tm_tm _ _ _ Eq_tm) s0)
   end.
 
-Lemma up_subst_ren_tm_tm {k : nat} {l_tm : nat} {m_tm : nat}
+Lemma up_subst_ren_tm_tm {k : list nat} {l_tm : list nat} {m_tm : list nat}
   (sigma : fin k -> tm l_tm) (zeta_tm : fin l_tm -> fin m_tm)
   (theta : fin k -> tm m_tm)
   (Eq : forall x, funcomp (ren_tm zeta_tm) sigma x = theta x) :
@@ -475,7 +333,7 @@ Lemma up_subst_ren_tm_tm {k : nat} {l_tm : nat} {m_tm : nat}
 Proof.
 exact (fun n =>
        match n with
-       | Some fin_n =>
+       | inr fin_n =>
            eq_trans
              (compRenRen_tm shift (upRen_tm_tm zeta_tm)
                 (funcomp shift zeta_tm) (fun x => eq_refl) (sigma fin_n))
@@ -484,35 +342,12 @@ exact (fun n =>
                    (compRenRen_tm zeta_tm shift (funcomp shift zeta_tm)
                       (fun x => eq_refl) (sigma fin_n)))
                 (ap (ren_tm shift) (Eq fin_n)))
-       | None => eq_refl
+       | inl n => eq_refl
        end).
 Qed.
 
-Lemma up_subst_ren_list_tm_tm {p : nat} {k : nat} {l_tm : nat} {m_tm : nat}
-  (sigma : fin k -> tm l_tm) (zeta_tm : fin l_tm -> fin m_tm)
-  (theta : fin k -> tm m_tm)
-  (Eq : forall x, funcomp (ren_tm zeta_tm) sigma x = theta x) :
-  forall x,
-  funcomp (ren_tm (upRen_list_tm_tm p zeta_tm)) (up_list_tm_tm p sigma) x =
-  up_list_tm_tm p theta x.
-Proof.
-exact (fun n =>
-       eq_trans (scons_p_comp' _ _ _ n)
-         (scons_p_congr
-            (fun x => ap (var_tm (plus p m_tm)) (scons_p_head' _ _ x))
-            (fun n =>
-             eq_trans
-               (compRenRen_tm (shift_p p) (upRen_list_tm_tm p zeta_tm)
-                  (funcomp (shift_p p) zeta_tm)
-                  (fun x => scons_p_tail' _ _ x) (sigma n))
-               (eq_trans
-                  (eq_sym
-                     (compRenRen_tm zeta_tm (shift_p p)
-                        (funcomp (shift_p p) zeta_tm) (fun x => eq_refl)
-                        (sigma n))) (ap (ren_tm (shift_p p)) (Eq n)))))).
-Qed.
 
-Fixpoint compSubstRen_tm {k_tm : nat} {l_tm : nat} {m_tm : nat}
+Fixpoint compSubstRen_tm {k_tm : list nat} {l_tm : list nat} {m_tm : list nat}
 (sigma_tm : fin m_tm -> tm k_tm) (zeta_tm : fin k_tm -> fin l_tm)
 (theta_tm : fin m_tm -> tm l_tm)
 (Eq_tm : forall x, funcomp (ren_tm zeta_tm) sigma_tm x = theta_tm x)
@@ -529,7 +364,7 @@ ren_tm zeta_tm (subst_tm sigma_tm s) = subst_tm theta_tm s :=
            (up_tm_tm theta_tm) (up_subst_ren_tm_tm _ _ _ Eq_tm) s0)
   end.
 
-Lemma up_subst_subst_tm_tm {k : nat} {l_tm : nat} {m_tm : nat}
+Lemma up_subst_subst_tm_tm {k : list nat} {l_tm : list nat} {m_tm : list nat}
   (sigma : fin k -> tm l_tm) (tau_tm : fin l_tm -> tm m_tm)
   (theta : fin k -> tm m_tm)
   (Eq : forall x, funcomp (subst_tm tau_tm) sigma x = theta x) :
@@ -538,7 +373,7 @@ Lemma up_subst_subst_tm_tm {k : nat} {l_tm : nat} {m_tm : nat}
 Proof.
 exact (fun n =>
        match n with
-       | Some fin_n =>
+       | inr fin_n =>
            eq_trans
              (compRenSubst_tm shift (up_tm_tm tau_tm)
                 (funcomp (up_tm_tm tau_tm) shift) (fun x => eq_refl)
@@ -548,36 +383,12 @@ exact (fun n =>
                    (compSubstRen_tm tau_tm shift
                       (funcomp (ren_tm shift) tau_tm) (fun x => eq_refl)
                       (sigma fin_n))) (ap (ren_tm shift) (Eq fin_n)))
-       | None => eq_refl
+       | inl n => eq_refl
        end).
 Qed.
 
-Lemma up_subst_subst_list_tm_tm {p : nat} {k : nat} {l_tm : nat} {m_tm : nat}
-  (sigma : fin k -> tm l_tm) (tau_tm : fin l_tm -> tm m_tm)
-  (theta : fin k -> tm m_tm)
-  (Eq : forall x, funcomp (subst_tm tau_tm) sigma x = theta x) :
-  forall x,
-  funcomp (subst_tm (up_list_tm_tm p tau_tm)) (up_list_tm_tm p sigma) x =
-  up_list_tm_tm p theta x.
-Proof.
-exact (fun n =>
-       eq_trans
-         (scons_p_comp' (funcomp (var_tm (plus p l_tm)) (zero_p p)) _ _ n)
-         (scons_p_congr
-            (fun x => scons_p_head' _ (fun z => ren_tm (shift_p p) _) x)
-            (fun n =>
-             eq_trans
-               (compRenSubst_tm (shift_p p) (up_list_tm_tm p tau_tm)
-                  (funcomp (up_list_tm_tm p tau_tm) (shift_p p))
-                  (fun x => eq_refl) (sigma n))
-               (eq_trans
-                  (eq_sym
-                     (compSubstRen_tm tau_tm (shift_p p) _
-                        (fun x => eq_sym (scons_p_tail' _ _ x)) (sigma n)))
-                  (ap (ren_tm (shift_p p)) (Eq n)))))).
-Qed.
 
-Fixpoint compSubstSubst_tm {k_tm : nat} {l_tm : nat} {m_tm : nat}
+Fixpoint compSubstSubst_tm {k_tm : list nat} {l_tm : list nat} {m_tm : list nat}
 (sigma_tm : fin m_tm -> tm k_tm) (tau_tm : fin k_tm -> tm l_tm)
 (theta_tm : fin m_tm -> tm l_tm)
 (Eq_tm : forall x, funcomp (subst_tm tau_tm) sigma_tm x = theta_tm x)
@@ -594,32 +405,20 @@ subst_tm tau_tm (subst_tm sigma_tm s) = subst_tm theta_tm s :=
            (up_tm_tm theta_tm) (up_subst_subst_tm_tm _ _ _ Eq_tm) s0)
   end.
 
-Lemma rinstInst_up_tm_tm {m : nat} {n_tm : nat} (xi : fin m -> fin n_tm)
+Lemma rinstInst_up_tm_tm {m : list nat} {n_tm : list nat} (xi : fin m -> fin n_tm)
   (sigma : fin m -> tm n_tm)
   (Eq : forall x, funcomp (var_tm n_tm) xi x = sigma x) :
-  forall x, funcomp (var_tm (S n_tm)) (upRen_tm_tm xi) x = up_tm_tm sigma x.
+  forall x, funcomp (var_tm (upT n_tm)) (upRen_tm_tm xi) x = up_tm_tm sigma x.
 Proof.
 exact (fun n =>
        match n with
-       | Some fin_n => ap (ren_tm shift) (Eq fin_n)
-       | None => eq_refl
+       | inr fin_n => ap (ren_tm shift) (Eq fin_n)
+       | inl n => eq_refl
        end).
 Qed.
 
-Lemma rinstInst_up_list_tm_tm {p : nat} {m : nat} {n_tm : nat}
-  (xi : fin m -> fin n_tm) (sigma : fin m -> tm n_tm)
-  (Eq : forall x, funcomp (var_tm n_tm) xi x = sigma x) :
-  forall x,
-  funcomp (var_tm (plus p n_tm)) (upRen_list_tm_tm p xi) x =
-  up_list_tm_tm p sigma x.
-Proof.
-exact (fun n =>
-       eq_trans (scons_p_comp' _ _ (var_tm (plus p n_tm)) n)
-         (scons_p_congr (fun z => eq_refl)
-            (fun n => ap (ren_tm (shift_p p)) (Eq n)))).
-Qed.
 
-Fixpoint rinst_inst_tm {m_tm : nat} {n_tm : nat}
+Fixpoint rinst_inst_tm {m_tm : list nat} {n_tm : list nat}
 (xi_tm : fin m_tm -> fin n_tm) (sigma_tm : fin m_tm -> tm n_tm)
 (Eq_tm : forall x, funcomp (var_tm n_tm) xi_tm x = sigma_tm x) (s : tm m_tm)
 {struct s} : ren_tm xi_tm s = subst_tm sigma_tm s :=
@@ -634,7 +433,7 @@ Fixpoint rinst_inst_tm {m_tm : nat} {n_tm : nat}
            (rinstInst_up_tm_tm _ _ Eq_tm) s0)
   end.
 
-Lemma renRen_tm {k_tm : nat} {l_tm : nat} {m_tm : nat}
+Lemma renRen_tm {k_tm : list nat} {l_tm : list nat} {m_tm : list nat}
   (xi_tm : fin m_tm -> fin k_tm) (zeta_tm : fin k_tm -> fin l_tm)
   (s : tm m_tm) :
   ren_tm zeta_tm (ren_tm xi_tm s) = ren_tm (funcomp zeta_tm xi_tm) s.
@@ -642,7 +441,9 @@ Proof.
 exact (compRenRen_tm xi_tm zeta_tm _ (fun n => eq_refl) s).
 Qed.
 
-Lemma renRen'_tm_pointwise {k_tm : nat} {l_tm : nat} {m_tm : nat}
+Require Import Setoid Morphisms.
+
+Lemma renRen'_tm_pointwise {k_tm : list nat} {l_tm : list nat} {m_tm : list nat}
   (xi_tm : fin m_tm -> fin k_tm) (zeta_tm : fin k_tm -> fin l_tm) :
   pointwise_relation _ eq (funcomp (ren_tm zeta_tm) (ren_tm xi_tm))
     (ren_tm (funcomp zeta_tm xi_tm)).
@@ -650,7 +451,7 @@ Proof.
 exact (fun s => compRenRen_tm xi_tm zeta_tm _ (fun n => eq_refl) s).
 Qed.
 
-Lemma substRen_tm {k_tm : nat} {l_tm : nat} {m_tm : nat}
+Lemma substRen_tm {k_tm : list nat} {l_tm : list nat} {m_tm : list nat}
   (sigma_tm : fin m_tm -> tm k_tm) (zeta_tm : fin k_tm -> fin l_tm)
   (s : tm m_tm) :
   ren_tm zeta_tm (subst_tm sigma_tm s) =
@@ -659,7 +460,7 @@ Proof.
 exact (compSubstRen_tm sigma_tm zeta_tm _ (fun n => eq_refl) s).
 Qed.
 
-Lemma substRen_tm_pointwise {k_tm : nat} {l_tm : nat} {m_tm : nat}
+Lemma substRen_tm_pointwise {k_tm : list nat} {l_tm : list nat} {m_tm : list nat}
   (sigma_tm : fin m_tm -> tm k_tm) (zeta_tm : fin k_tm -> fin l_tm) :
   pointwise_relation _ eq (funcomp (ren_tm zeta_tm) (subst_tm sigma_tm))
     (subst_tm (funcomp (ren_tm zeta_tm) sigma_tm)).
@@ -667,14 +468,14 @@ Proof.
 exact (fun s => compSubstRen_tm sigma_tm zeta_tm _ (fun n => eq_refl) s).
 Qed.
 
-Lemma renSubst_tm {k_tm : nat} {l_tm : nat} {m_tm : nat}
+Lemma renSubst_tm {k_tm : list nat} {l_tm : list nat} {m_tm : list nat}
   (xi_tm : fin m_tm -> fin k_tm) (tau_tm : fin k_tm -> tm l_tm) (s : tm m_tm)
   : subst_tm tau_tm (ren_tm xi_tm s) = subst_tm (funcomp tau_tm xi_tm) s.
 Proof.
 exact (compRenSubst_tm xi_tm tau_tm _ (fun n => eq_refl) s).
 Qed.
 
-Lemma renSubst_tm_pointwise {k_tm : nat} {l_tm : nat} {m_tm : nat}
+Lemma renSubst_tm_pointwise {k_tm : list nat} {l_tm : list nat} {m_tm : list nat}
   (xi_tm : fin m_tm -> fin k_tm) (tau_tm : fin k_tm -> tm l_tm) :
   pointwise_relation _ eq (funcomp (subst_tm tau_tm) (ren_tm xi_tm))
     (subst_tm (funcomp tau_tm xi_tm)).
@@ -682,7 +483,7 @@ Proof.
 exact (fun s => compRenSubst_tm xi_tm tau_tm _ (fun n => eq_refl) s).
 Qed.
 
-Lemma substSubst_tm {k_tm : nat} {l_tm : nat} {m_tm : nat}
+Lemma substSubst_tm {k_tm : list nat} {l_tm : list nat} {m_tm : list nat}
   (sigma_tm : fin m_tm -> tm k_tm) (tau_tm : fin k_tm -> tm l_tm)
   (s : tm m_tm) :
   subst_tm tau_tm (subst_tm sigma_tm s) =
@@ -691,7 +492,7 @@ Proof.
 exact (compSubstSubst_tm sigma_tm tau_tm _ (fun n => eq_refl) s).
 Qed.
 
-Lemma substSubst_tm_pointwise {k_tm : nat} {l_tm : nat} {m_tm : nat}
+Lemma substSubst_tm_pointwise {k_tm : list nat} {l_tm : list nat} {m_tm : list nat}
   (sigma_tm : fin m_tm -> tm k_tm) (tau_tm : fin k_tm -> tm l_tm) :
   pointwise_relation _ eq (funcomp (subst_tm tau_tm) (subst_tm sigma_tm))
     (subst_tm (funcomp (subst_tm tau_tm) sigma_tm)).
@@ -699,13 +500,13 @@ Proof.
 exact (fun s => compSubstSubst_tm sigma_tm tau_tm _ (fun n => eq_refl) s).
 Qed.
 
-Lemma rinstInst'_tm {m_tm : nat} {n_tm : nat} (xi_tm : fin m_tm -> fin n_tm)
+Lemma rinstInst'_tm {m_tm : list nat} {n_tm : list nat} (xi_tm : fin m_tm -> fin n_tm)
   (s : tm m_tm) : ren_tm xi_tm s = subst_tm (funcomp (var_tm n_tm) xi_tm) s.
 Proof.
 exact (rinst_inst_tm xi_tm _ (fun n => eq_refl) s).
 Qed.
 
-Lemma rinstInst'_tm_pointwise {m_tm : nat} {n_tm : nat}
+Lemma rinstInst'_tm_pointwise {m_tm : list nat} {n_tm : list nat}
   (xi_tm : fin m_tm -> fin n_tm) :
   pointwise_relation _ eq (ren_tm xi_tm)
     (subst_tm (funcomp (var_tm n_tm) xi_tm)).
@@ -713,35 +514,35 @@ Proof.
 exact (fun s => rinst_inst_tm xi_tm _ (fun n => eq_refl) s).
 Qed.
 
-Lemma instId'_tm {m_tm : nat} (s : tm m_tm) : subst_tm (var_tm m_tm) s = s.
+Lemma instId'_tm {m_tm : list nat} (s : tm m_tm) : subst_tm (var_tm m_tm) s = s.
 Proof.
 exact (idSubst_tm (var_tm m_tm) (fun n => eq_refl) s).
 Qed.
 
-Lemma instId'_tm_pointwise {m_tm : nat} :
+Lemma instId'_tm_pointwise {m_tm : list nat} :
   pointwise_relation _ eq (subst_tm (var_tm m_tm)) id.
 Proof.
 exact (fun s => idSubst_tm (var_tm m_tm) (fun n => eq_refl) s).
 Qed.
 
-Lemma rinstId'_tm {m_tm : nat} (s : tm m_tm) : ren_tm id s = s.
+Lemma rinstId'_tm {m_tm : list nat} (s : tm m_tm) : ren_tm id s = s.
 Proof.
 exact (eq_ind_r (fun t => t = s) (instId'_tm s) (rinstInst'_tm id s)).
 Qed.
 
-Lemma rinstId'_tm_pointwise {m_tm : nat} :
+Lemma rinstId'_tm_pointwise {m_tm : list nat} :
   pointwise_relation _ eq (@ren_tm m_tm m_tm id) id.
 Proof.
 exact (fun s => eq_ind_r (fun t => t = s) (instId'_tm s) (rinstInst'_tm id s)).
 Qed.
 
-Lemma varL'_tm {m_tm : nat} {n_tm : nat} (sigma_tm : fin m_tm -> tm n_tm)
+Lemma varL'_tm {m_tm : list nat} {n_tm : list nat} (sigma_tm : fin m_tm -> tm n_tm)
   (x : fin m_tm) : subst_tm sigma_tm (var_tm m_tm x) = sigma_tm x.
 Proof.
 exact (eq_refl).
 Qed.
 
-Lemma varL'_tm_pointwise {m_tm : nat} {n_tm : nat}
+Lemma varL'_tm_pointwise {m_tm : list nat} {n_tm : list nat}
   (sigma_tm : fin m_tm -> tm n_tm) :
   pointwise_relation _ eq (funcomp (subst_tm sigma_tm) (var_tm m_tm))
     sigma_tm.
@@ -749,13 +550,13 @@ Proof.
 exact (fun x => eq_refl).
 Qed.
 
-Lemma varLRen'_tm {m_tm : nat} {n_tm : nat} (xi_tm : fin m_tm -> fin n_tm)
+Lemma varLRen'_tm {m_tm : list nat} {n_tm : list nat} (xi_tm : fin m_tm -> fin n_tm)
   (x : fin m_tm) : ren_tm xi_tm (var_tm m_tm x) = var_tm n_tm (xi_tm x).
 Proof.
 exact (eq_refl).
 Qed.
 
-Lemma varLRen'_tm_pointwise {m_tm : nat} {n_tm : nat}
+Lemma varLRen'_tm_pointwise {m_tm : list nat} {n_tm : list nat}
   (xi_tm : fin m_tm -> fin n_tm) :
   pointwise_relation _ eq (funcomp (ren_tm xi_tm) (var_tm m_tm))
     (funcomp (var_tm n_tm) xi_tm).
@@ -763,42 +564,42 @@ Proof.
 exact (fun x => eq_refl).
 Qed.
 
-Class Up_tm X Y :=
-    up_tm : X -> Y.
+(* Class Up_tm X Y := *)
+(*     up_tm : X -> Y. *)
 
-Instance Subst_tm  {m_tm n_tm : nat}: (Subst1 _ _ _) := (@subst_tm m_tm n_tm).
+(* Instance Subst_tm  {m_tm n_tm : nat}: (Subst1 _ _ _) := (@subst_tm m_tm n_tm). *)
 
-Instance Up_tm_tm  {m n_tm : nat}: (Up_tm _ _) := (@up_tm_tm m n_tm).
+(* Instance Up_tm_tm  {m n_tm : nat}: (Up_tm _ _) := (@up_tm_tm m n_tm). *)
 
-Instance Ren_tm  {m_tm n_tm : nat}: (Ren1 _ _ _) := (@ren_tm m_tm n_tm).
+(* Instance Ren_tm  {m_tm n_tm : nat}: (Ren1 _ _ _) := (@ren_tm m_tm n_tm). *)
 
-Instance VarInstance_tm  {n_tm : nat}: (Var _ _) := (@var_tm n_tm).
+(* Instance VarInstance_tm  {n_tm : nat}: (Var _ _) := (@var_tm n_tm). *)
 
-Notation "[ sigma_tm ]" := (subst_tm sigma_tm)
-  ( at level 1, left associativity, only printing) : fscope.
+(* Notation "[ sigma_tm ]" := (subst_tm sigma_tm) *)
+(*   ( at level 1, left associativity, only printing) : fscope. *)
 
-Notation "s [ sigma_tm ]" := (subst_tm sigma_tm s)
-  ( at level 7, left associativity, only printing) : subst_scope.
+(* Notation "s [ sigma_tm ]" := (subst_tm sigma_tm s) *)
+(*   ( at level 7, left associativity, only printing) : subst_scope. *)
 
-Notation "↑__tm" := up_tm (only printing) : subst_scope.
+(* Notation "↑__tm" := up_tm (only printing) : subst_scope. *)
 
-Notation "↑__tm" := up_tm_tm (only printing) : subst_scope.
+(* Notation "↑__tm" := up_tm_tm (only printing) : subst_scope. *)
 
-Notation "⟨ xi_tm ⟩" := (ren_tm xi_tm)
-  ( at level 1, left associativity, only printing) : fscope.
+(* Notation "⟨ xi_tm ⟩" := (ren_tm xi_tm) *)
+(*   ( at level 1, left associativity, only printing) : fscope. *)
 
-Notation "s ⟨ xi_tm ⟩" := (ren_tm xi_tm s)
-  ( at level 7, left associativity, only printing) : subst_scope.
+(* Notation "s ⟨ xi_tm ⟩" := (ren_tm xi_tm s) *)
+(*   ( at level 7, left associativity, only printing) : subst_scope. *)
 
-Notation "'var'" := var_tm ( at level 1, only printing) : subst_scope.
+(* Notation "'var'" := var_tm ( at level 1, only printing) : subst_scope. *)
 
-Notation "x '__tm'" := (@ids _ _ VarInstance_tm x)
-  ( at level 5, format "x __tm", only printing) : subst_scope.
+(* Notation "x '__tm'" := (@ids _ _ VarInstance_tm x) *)
+(*   ( at level 5, format "x __tm", only printing) : subst_scope. *)
 
-Notation "x '__tm'" := (var_tm x) ( at level 5, format "x __tm") :
-  subst_scope.
+(* Notation "x '__tm'" := (var_tm x) ( at level 5, format "x __tm") : *)
+(*   subst_scope. *)
 
-Instance subst_tm_morphism  {m_tm : nat} {n_tm : nat}:
+Instance subst_tm_morphism  {m_tm : list nat} {n_tm : list nat}:
  (Proper (respectful (pointwise_relation _ eq) (respectful eq eq))
     (@subst_tm m_tm n_tm)).
 Proof.
@@ -807,7 +608,7 @@ exact (fun f_tm g_tm Eq_tm s t Eq_st =>
          (ext_tm f_tm g_tm Eq_tm s) t Eq_st).
 Qed.
 
-Instance ren_tm_morphism  {m_tm : nat} {n_tm : nat}:
+Instance ren_tm_morphism  {m_tm : list nat} {n_tm : list nat}:
  (Proper (respectful (pointwise_relation _ eq) (respectful eq eq))
     (@ren_tm m_tm n_tm)).
 Proof.
@@ -816,15 +617,15 @@ exact (fun f_tm g_tm Eq_tm s t Eq_st =>
          (extRen_tm f_tm g_tm Eq_tm s) t Eq_st).
 Qed.
 
-Ltac auto_unfold := repeat
-                     unfold VarInstance_tm, Var, ids, Ren_tm, Ren1, ren1,
-                      Up_tm_tm, Up_tm, up_tm, Subst_tm, Subst1, subst1.
+(* Ltac auto_unfold := repeat *)
+(*                      unfold VarInstance_tm, Var, ids, Ren_tm, Ren1, ren1, *)
+(*                       Up_tm_tm, Up_tm, up_tm, Subst_tm, Subst1, subst1. *)
 
-Tactic Notation "auto_unfold" "in" "*" := repeat
-                                           unfold VarInstance_tm, Var, ids,
-                                            Ren_tm, Ren1, ren1, Up_tm_tm,
-                                            Up_tm, up_tm, Subst_tm, Subst1,
-                                            subst1 in *.
+(* Tactic Notation "auto_unfold" "in" "*" := repeat *)
+(*                                            unfold VarInstance_tm, Var, ids, *)
+(*                                             Ren_tm, Ren1, ren1, Up_tm_tm, *)
+(*                                             Up_tm, up_tm, Subst_tm, Subst1, *)
+(*                                             subst1 in *. *)
 
 Ltac asimpl' := repeat (first
                  [ progress setoid_rewrite substSubst_tm_pointwise
@@ -844,26 +645,12 @@ Ltac asimpl' := repeat (first
                  | progress setoid_rewrite instId'_tm_pointwise
                  | progress setoid_rewrite instId'_tm
                  | progress
-                    unfold up_list_tm_tm, up_tm_tm, upRen_list_tm_tm,
+                    unfold up_tm_tm, 
                      upRen_tm_tm, up_ren
                  | progress cbn[subst_tm ren_tm]
-                 | progress fsimpl ]).
+                   ]).
 
-Ltac asimpl := check_no_evars;
-                repeat
-                 unfold VarInstance_tm, Var, ids, Ren_tm, Ren1, ren1,
-                  Up_tm_tm, Up_tm, up_tm, Subst_tm, Subst1, subst1 in *;
-                asimpl'; minimize.
 
-Tactic Notation "asimpl" "in" hyp(J) := revert J; asimpl; intros J.
-
-Tactic Notation "auto_case" := auto_case ltac:(asimpl; cbn; eauto).
-
-Ltac substify := auto_unfold; try setoid_rewrite rinstInst'_tm_pointwise;
-                  try setoid_rewrite rinstInst'_tm.
-
-Ltac renamify := auto_unfold; try setoid_rewrite_left rinstInst'_tm_pointwise;
-                  try setoid_rewrite_left rinstInst'_tm.
 
 End renSubst.
 
@@ -872,39 +659,41 @@ Module fext.
 Import
 renSubst.
 
-Lemma rinstInst_tm {m_tm : nat} {n_tm : nat} (xi_tm : fin m_tm -> fin n_tm) :
+Require Import Coq.Logic.FunctionalExtensionality.
+
+Lemma rinstInst_tm {m_tm : list nat} {n_tm : list nat} (xi_tm : fin m_tm -> fin n_tm) :
   ren_tm xi_tm = subst_tm (funcomp (var_tm n_tm) xi_tm).
 Proof.
 exact (FunctionalExtensionality.functional_extensionality _ _
          (fun x => rinst_inst_tm xi_tm _ (fun n => eq_refl) x)).
 Qed.
 
-Lemma instId_tm {m_tm : nat} : subst_tm (var_tm m_tm) = id.
+Lemma instId_tm {m_tm : list nat} : subst_tm (var_tm m_tm) = id.
 Proof.
 exact (FunctionalExtensionality.functional_extensionality _ _
          (fun x => idSubst_tm (var_tm m_tm) (fun n => eq_refl) (id x))).
 Qed.
 
-Lemma rinstId_tm {m_tm : nat} : @ren_tm m_tm m_tm id = id.
+Lemma rinstId_tm {m_tm : list nat} : @ren_tm m_tm m_tm id = id.
 Proof.
 exact (eq_trans (rinstInst_tm (id _)) instId_tm).
 Qed.
 
-Lemma varL_tm {m_tm : nat} {n_tm : nat} (sigma_tm : fin m_tm -> tm n_tm) :
+Lemma varL_tm {m_tm : list nat} {n_tm : list nat} (sigma_tm : fin m_tm -> tm n_tm) :
   funcomp (subst_tm sigma_tm) (var_tm m_tm) = sigma_tm.
 Proof.
 exact (FunctionalExtensionality.functional_extensionality _ _
          (fun x => eq_refl)).
 Qed.
 
-Lemma varLRen_tm {m_tm : nat} {n_tm : nat} (xi_tm : fin m_tm -> fin n_tm) :
+Lemma varLRen_tm {m_tm : list nat} {n_tm : list nat} (xi_tm : fin m_tm -> fin n_tm) :
   funcomp (ren_tm xi_tm) (var_tm m_tm) = funcomp (var_tm n_tm) xi_tm.
 Proof.
 exact (FunctionalExtensionality.functional_extensionality _ _
          (fun x => eq_refl)).
 Qed.
 
-Lemma renRen'_tm {k_tm : nat} {l_tm : nat} {m_tm : nat}
+Lemma renRen'_tm {k_tm : list nat} {l_tm : list nat} {m_tm : list nat}
   (xi_tm : fin m_tm -> fin k_tm) (zeta_tm : fin k_tm -> fin l_tm) :
   funcomp (ren_tm zeta_tm) (ren_tm xi_tm) = ren_tm (funcomp zeta_tm xi_tm).
 Proof.
@@ -912,7 +701,7 @@ exact (FunctionalExtensionality.functional_extensionality _ _
          (fun n => renRen_tm xi_tm zeta_tm n)).
 Qed.
 
-Lemma substRen'_tm {k_tm : nat} {l_tm : nat} {m_tm : nat}
+Lemma substRen'_tm {k_tm : list nat} {l_tm : list nat} {m_tm : list nat}
   (sigma_tm : fin m_tm -> tm k_tm) (zeta_tm : fin k_tm -> fin l_tm) :
   funcomp (ren_tm zeta_tm) (subst_tm sigma_tm) =
   subst_tm (funcomp (ren_tm zeta_tm) sigma_tm).
@@ -921,7 +710,7 @@ exact (FunctionalExtensionality.functional_extensionality _ _
          (fun n => substRen_tm sigma_tm zeta_tm n)).
 Qed.
 
-Lemma renSubst'_tm {k_tm : nat} {l_tm : nat} {m_tm : nat}
+Lemma renSubst'_tm {k_tm : list nat} {l_tm : list nat} {m_tm : list nat}
   (xi_tm : fin m_tm -> fin k_tm) (tau_tm : fin k_tm -> tm l_tm) :
   funcomp (subst_tm tau_tm) (ren_tm xi_tm) = subst_tm (funcomp tau_tm xi_tm).
 Proof.
@@ -929,7 +718,7 @@ exact (FunctionalExtensionality.functional_extensionality _ _
          (fun n => renSubst_tm xi_tm tau_tm n)).
 Qed.
 
-Lemma substSubst'_tm {k_tm : nat} {l_tm : nat} {m_tm : nat}
+Lemma substSubst'_tm {k_tm : list nat} {l_tm : list nat} {m_tm : list nat}
   (sigma_tm : fin m_tm -> tm k_tm) (tau_tm : fin k_tm -> tm l_tm) :
   funcomp (subst_tm tau_tm) (subst_tm sigma_tm) =
   subst_tm (funcomp (subst_tm tau_tm) sigma_tm).
@@ -956,22 +745,10 @@ Ltac asimpl_fext' := repeat (first
                       | progress setoid_rewrite rinstId_tm
                       | progress setoid_rewrite instId_tm
                       | progress
-                         unfold up_list_tm_tm, up_tm_tm, upRen_list_tm_tm,
+                         unfold up_tm_tm, 
                           upRen_tm_tm, up_ren
-                      | progress cbn[subst_tm ren_tm]
-                      | fsimpl_fext ]).
+                      | progress cbn[subst_tm ren_tm] ]).
 
-Ltac asimpl_fext := check_no_evars; repeat try unfold_funcomp;
-                     repeat
-                      unfold VarInstance_tm, Var, ids, Ren_tm, Ren1, ren1,
-                       Up_tm_tm, Up_tm, up_tm, Subst_tm, Subst1, subst1 
-                       in *; asimpl_fext'; repeat try unfold_funcomp.
-
-Tactic Notation "asimpl_fext" "in" hyp(J) := revert J; asimpl_fext; intros J.
-
-Ltac substify_fext := auto_unfold; try repeat erewrite ?rinstInst_tm.
-
-Ltac renamify_fext := auto_unfold; try repeat erewrite <- ?rinstInst_tm.
 
 End fext.
 
@@ -982,11 +759,11 @@ Export renSubst.
 Export
 fext.
 
-Arguments var_tm {n_tm}.
+Arguments var_tm {vs}.
 
-Arguments lam {n_tm}.
+Arguments lam {vs}.
 
-Arguments app {n_tm}.
+Arguments app {vs}.
 
 Hint Opaque subst_tm: rewrite.
 
