case-studies/kathrin/coq/Chapter9/sn.v
@@ -59,9 +59,7 @@ Proof.
   induction A; eauto.
   destruct s; try contradiction.
   subst. intros. cbn in *. intros. asimpl.
-  (* TODO eauto does not work but we can simply apply both assumptions. But why does it not work? *)
-  apply H, H0.
-  (* eauto. *)
+  eauto.
 Qed.
 
 Lemma close_ren  :
